lean-formalisation/LeanFormalisation/LBaseCFG/alt/Framework.lean
@@ -1,0 +1,30 @@
+import LeanFormalisation.LBaseCFG.alt.AltCFG
+import LeanFormalisation.LBaseCFG.alt.Analysis
+
+open LeanFormalisation.AltCFG
+
+/-- An analysis `Framework` is a structure comprised of
+    - a lattice-like abstract domain `A`,
+    - transfer functions describing the update to the domain based on the
+      CFG state
+    - an abstraction function to turn a concrete state to an element of the
+      abstract domain
+
+    Additionally, we guarantee regular lattice properties on `A`, and
+    monotonicity with respect to it of the transfer functions.
+-/
+class Framework
+    (A : Type) [Bot A] [Max A]
+    (edgeTransfer : CFGEdge -> A -> A)
+    (nodeTransfer : CFGNode -> A -> A)
+    (abs : CEK -> A -> Prop) where
+
+  -- regular lattice structure
+  join_comm : ∀ a b : A, a ⊔ b = b ⊔ a
+  join_assoc : ∀ a b c : A, (a ⊔ b) ⊔ c = a ⊔ (b ⊔ c)
+  join_idem : ∀ a : A, a ⊔ a = a
+  bot_le : ∀ a : A, a ⊔ ⊥ = a
+
+  -- monotonicity of the transfer
+  node_mono : ∀ n, monotoneD (nodeTransfer n)
+  edge_mono : ∀ e, monotoneD (edgeTransfer e)
